Calculation of the determinant:
\alg{
  \nabla_{\Bc_m}\left\{\det \BF(X,t)\right\}
  &=\nabla_{\Bc_m}\left\{\det \left( \sumlim{i=1}{N}{\Bc_i(t) \otimes \nabla \varphi_i(X)} \right) \right\} \nonumber\\
  &=\nabla_{\Bc_m}\left\{\det \left( \sumlim{i=1}{N}{
      \begin{bmatrix}
        c_{i1} \varphi_{i,1}  & c_{i1} \varphi_{i,2}  & c_{i1} \varphi_{i,3} \\
        c_{i2} \varphi_{i,1}  & c_{i2} \varphi_{i,2}  & c_{i2} \varphi_{i,3} \\
        c_{i3} \varphi_{i,1}  & c_{i3} \varphi_{i,2}  & c_{i3} \varphi_{i,3}
      \end{bmatrix}
    } \right) \right\} \nonumber\\
  &=\nabla_{\Bc_m}\Bigg\{
      \left( \sumlim{i=1}{N}{c_{i1}\varphi_{i,1}}\right) \left[
        \left( \sumlim{i=1}{N}{c_{i2}\varphi_{i,2}}\right) \left( \sumlim{i=1}{N}{c_{i3}\varphi_{i,3}}\right)
        - \left( \sumlim{i=1}{N}{c_{i2}\varphi_{i,3}}\right) \left( \sumlim{i=1}{N}{c_{i3}\varphi_{i,2}}\right)
      \right]
      \nonumber\\
      &\hspace{11.5mm} -\left( \sumlim{i=1}{N}{c_{i1}\varphi_{i,2}}\right) \left[
        \left( \sumlim{i=1}{N}{c_{i2}\varphi_{i,1}}\right) \left( \sumlim{i=1}{N}{c_{i3}\varphi_{i,3}}\right)
        - \left( \sumlim{i=1}{N}{c_{i2}\varphi_{i,3}}\right) \left( \sumlim{i=1}{N}{c_{i3}\varphi_{i,1}}\right)
      \right]
      \nonumber\\
      &\hspace{11.5mm} +\left( \sumlim{i=1}{N}{c_{i1}\varphi_{i,3}}\right) \left[
        \left( \sumlim{i=1}{N}{c_{i2}\varphi_{i,1}}\right) \left( \sumlim{i=1}{N}{c_{i3}\varphi_{i,2}}\right)
        - \left( \sumlim{i=1}{N}{c_{i2}\varphi_{i,2}}\right) \left( \sumlim{i=1}{N}{c_{i3}\varphi_{i,1}}\right)
      \right]
    \Bigg\}\nonumber\\
  &=\nabla_{\Bc_m}\Bigg\{
  \sumlim{i,j,k=1}{N}{c_{i1} \varphi_{i,1} \, c_{j2} \varphi_{j,2} \, c_{k3}\varphi_{k,3}}
    -\sumlim{i,j,k=1}{N}{c_{i1} \varphi_{i,1} \, c_{j2} \varphi_{j,3} \, c_{k3}\varphi_{k,2}}
    \nonumber\\
    &\hspace{11.5mm}-\sumlim{i,j,k=1}{N}{c_{i1} \varphi_{i,2} \, c_{j2} \varphi_{j,1} \, c_{k3}\varphi_{k,3}}
    +\sumlim{i,j,k=1}{N}{c_{i1} \varphi_{i,2} \, c_{j2} \varphi_{j,3} \, c_{k3}\varphi_{k,1}}
    \nonumber\\
    &\hspace{11.5mm}+\sumlim{i,j,k=1}{N}{c_{i1} \varphi_{i,3} \, c_{j2} \varphi_{j,1} \, c_{k3}\varphi_{k,2}}
    -\sumlim{i,j,k=1}{N}{c_{i1} \varphi_{i,3} \, c_{j2} \varphi_{j,2} \, c_{k3}\varphi_{k,1}} 
    \Bigg\}\nonumber\\
  &=\nabla_{\Bc_m}\Bigg\{
    \sumlim{i,j,k=1}{N}{
    c_{i1} c_{j2} c_{k3} (
      \varphi_{i,1} \varphi_{j,2} \varphi_{k,3}-\varphi_{i,1} \varphi_{j,3} \varphi_{k,2}-\varphi_{i,2} \varphi_{j,1} \varphi_{k,3}
      }\nonumber\\
      &\hspace{20mm}+\varphi_{i,2} \varphi_{j,3} \varphi_{k,1}+\varphi_{i,3} \varphi_{j,1} \varphi_{k,2}
      -\varphi_{i,3} \varphi_{j,2} \varphi_{k,1} )
    \Bigg\}\nonumber\\
  &=\nabla_{\Bc_m}\Bigg\{
      \sumlim{i,j,k=1}{N}{
      c_{i1} c_{j2} c_{k3} 
      \det  \begin{bmatrix}
              \varphi_{i,1} & \varphi_{i,2} & \varphi_{i,3} \\
              \varphi_{j,1} & \varphi_{j,2} & \varphi_{j,3} \\
              \varphi_{k,1} & \varphi_{k,2} & \varphi_{k,3}
            \end{bmatrix}
      }
    \Bigg\} \nonumber\\
  &=\nabla_{\Bc_m}\Bigg\{
      \sumlim{i,j,k=1}{N}{
      c_{i1}(t) c_{j2}(t) c_{k3}(t)
      \det \begin{bmatrix}
              \nabla \varphi_{i}(X) \\
              \nabla \varphi_{j}(X) \\
              \nabla \varphi_{k}(X)
            \end{bmatrix}
      }
    \Bigg\}
}
%
%-------
\newpage
%-------
%
Calculation of the gradient:
\alg{
  \nabla_{\Bc_m}\left\{\det \BF(X,t)\right\}
  &=\nabla_{\Bc_m}\Bigg\{
      \sumlim{i,j,k=1}{N}{
      c_{i1}(t) c_{j2}(t) c_{k3}(t)
      \det \begin{bmatrix}
              \nabla \varphi_{i}(X) \\
              \nabla \varphi_{j}(X) \\
              \nabla \varphi_{k}(X)
            \end{bmatrix}
      }
    \Bigg\} \nonumber\\
  &=\sumlim{i,j,k=1}{N}{\left(
      \begin{bmatrix}
        \delby{c_{i1}}{c_{m1}}c_{j2}c_{k3} + c_{i1} \cancel{\delby{c_{j2}}{c_{m1}}} c_{k3} 
          + c_{i1}c_{j2}\cancel{\delby{c_{k3}}{c_{m1}}} \\
        \cancel{\delby{c_{i1}}{c_{m2}}}c_{j2}c_{k3} + c_{i1} \delby{c_{j2}}{c_{m2}} c_{k3} 
          + c_{i1}c_{j2}\cancel{\delby{c_{k3}}{c_{m2}}} \\
        \cancel{\delby{c_{i1}}{c_{m3}}}c_{j2}c_{k3} + c_{i1} \cancel{\delby{c_{j2}}{c_{m3}}} c_{k3} 
        + c_{i1}c_{j2}\delby{c_{k3}}{c_{m3}}
      \end{bmatrix}
      \det \begin{bmatrix}
              \nabla \varphi_{i}(X) \\
              \nabla \varphi_{j}(X) \\
              \nabla \varphi_{k}(X)
            \end{bmatrix}
      \right)}
      \nonumber\\
  &=\sumlim{i,j,k=1}{N}{\left(
      \begin{bmatrix}
        \delta_{im}c_{j2}c_{k3}\\
        c_{i1}\delta_{jm}c_{k3}\\
        c_{i1}c_{j2}\delta_{km}
      \end{bmatrix}
      \det \begin{bmatrix}
              \nabla \varphi_{i}(X) \\
              \nabla \varphi_{j}(X) \\
              \nabla \varphi_{k}(X)
            \end{bmatrix}
      \right)}
      \nonumber\\
  &=\begin{pmatrix}
      \sumlim{j,k=1}{N}{
        c_{j2}c_{k3} \det \begin{bmatrix}
                            \nabla \varphi_{m}(X) \\
                            \nabla \varphi_{j}(X) \\
                            \nabla \varphi_{k}(X)
                          \end{bmatrix}
      } \\
      \sumlim{i,k=1}{N}{
        c_{i1}c_{k3} \det \begin{bmatrix}
                            \nabla \varphi_{i}(X) \\
                            \nabla \varphi_{m}(X) \\
                            \nabla \varphi_{k}(X)
                          \end{bmatrix}
      } \\
      \sumlim{i,j=1}{N}{
        c_{i1}c_{j2} \det \begin{bmatrix}
                            \nabla \varphi_{i}(X) \\
                            \nabla \varphi_{j}(X) \\
                            \nabla \varphi_{m}(X)
                          \end{bmatrix}
      }            
    \end{pmatrix}
    \nonumber\\
  &=\sumlim{i,j=1}{N}{
      \begin{pmatrix}
        c_{i2}c_{j3}\det \begin{bmatrix}
                            \nabla \varphi_{m}(X) \\
                            \nabla \varphi_{i}(X) \\
                            \nabla \varphi_{j}(X)
                          \end{bmatrix}
        \\
        c_{i1}c_{j3}\det \begin{bmatrix}
                            \nabla \varphi_{i}(X) \\
                            \nabla \varphi_{m}(X) \\
                            \nabla \varphi_{j}(X)
                          \end{bmatrix}
        \\
        c_{i1}c_{j2}\det \begin{bmatrix}
                            \nabla \varphi_{i}(X) \\
                            \nabla \varphi_{j}(X) \\
                            \nabla \varphi_{m}(X)
                          \end{bmatrix}
      \end{pmatrix}
    }
    =:\ \begin{pmatrix}
          \nabla_{c_{m1}}\left\{\det \BF(X,t)\right\} \\
          \nabla_{c_{m2}}\left\{\det \BF(X,t)\right\} \\
          \nabla_{c_{m3}}\left\{\det \BF(X,t)\right\}                  
        \end{pmatrix}
}
%
%-------
\newpage
%-------
%
It holds that:
\beq{}
  \boxed{
  \det(\BS+\BU) = \det \BS + \det \BS (\BS^{T-1}:\BU) \,.
  }
\eeq
Furthermore, for the inverse of a matrix/tensor, it holds
\beq{}
  \BA^{-1} = (\det \BA)^{-1} \textnormal{adj}\BA
  \Longrightarrow
  \BA^{T-1} = (\det \BA)^{-1} \textnormal{cof}\BA \,,
\eeq
where
\beq{}
  \textnormal{cof}\BA = \textnormal{cof}
    \begin{pmatrix}
      A_{11}  & A_{12}  & A_{13} \\
      A_{21}  & A_{22}  & A_{23} \\
      A_{31}  & A_{32}  & A_{33}
    \end{pmatrix}
    = \begin{pmatrix}
        A_{22}A_{33}-A_{23}A_{32} & A_{23}A_{31}-A_{21}A_{33} & A_{21}A_{32}-A_{22}A_{31} \\
        A_{13}A_{32}-A_{12}A_{33} & A_{11}A_{33}-A_{13}A_{31} & A_{12}A_{31}-A_{11}A_{32} \\
        A_{12}A_{23}-A_{13}A_{22} & A_{13}A_{21}-A_{11}A_{23} & A_{11}A_{22}-A_{12}A_{21}
      \end{pmatrix} \,.
\eeq
"{\bf \underline{Lemma}}": \par
For $\BS:=\BF$ and $\BU:=\BU^m_l$, $l=1,2,3$, with
\beq{}
  \BU^m_1:= \begin{pmatrix}
            ~   & \nabla \varphi_m  & ~ \\
            0   & 0                 & 0 \\
            0   & 0                 & 0
          \end{pmatrix},\,
  \BU^m_2:= \begin{pmatrix}
            0   & 0                 & 0 \\
            ~   & \nabla \varphi_m  & ~ \\            
            0   & 0                 & 0
          \end{pmatrix},\,
  \BU^m_3:= \begin{pmatrix}
            0   & 0                 & 0 \\
            0   & 0                 & 0 \\
            ~   & \nabla \varphi_m  & ~            
          \end{pmatrix},          
\eeq
it holds that
\beq{}
  \boxed{
  \nabla_{c_{ml}}\left\{\det \BF(X,t)\right\} = \det \BF \left(\BF^{T-1}:\BU^m_l\right) \,.
  }
\eeq
"{\bf \underline{Proof}}": \par
Setting $l:=1$ yields:
\alg{
  \det \BF \left(\BF^{T-1}:\BU^m_1\right)
  &= \cancel{\det \BF (\det \BF)^{-1}} \textnormal{cof}\BF : \BU^m_1 \nonumber\\
  &= \textnormal{cof}\BF 
        \begin{pmatrix}
           ~   & \nabla \varphi_m  & ~ \\
           0   & 0                 & 0 \\
           0   & 0                 & 0
        \end{pmatrix}
    \nonumber\\
  &= \varphi_{m,1} (F_{22}F_{33}-F_{23}F_{32}) +
      \varphi_{m,2} (F_{23}F_{31}-F_{21}F_{33}) +
      \varphi_{m,3} (F_{21}F_{32}-F_{22}F_{31})
    \nonumber\\
  &= \varphi_{m,1} \left(
        \sumlim{i,j=1}{N}{c_{i2}\varphi_{i,2}c_{j3}\varphi_{j,3}}
        - \sumlim{i,j=1}{N}{c_{i2}\varphi_{i,3}c_{j3}\varphi_{j,2}}
      \right) \nonumber\\
    &\hspace{6mm}+\varphi_{m,2} \left(
        \sumlim{i,j=1}{N}{c_{i2}\varphi_{i,3}c_{j3}\varphi_{j,1}}
        - \sumlim{i,j=1}{N}{c_{i2}\varphi_{i,1}c_{j3}\varphi_{j,3}}
      \right)\nonumber\\
    &\hspace{6mm}+\varphi_{m,3} \left(
        \sumlim{i,j=1}{N}{c_{i2}\varphi_{i,1}c_{j3}\varphi_{j,2}}
        - \sumlim{i,j=1}{N}{c_{i2}\varphi_{i,2}c_{j3}\varphi_{j,1}}
      \right) \nonumber\\
  &= \sumlim{i,j=1}{N}{c_{i2}c_{j3}
      (
      \varphi_{m,1}\varphi_{i,2} \varphi_{j,3}-\varphi_{m,1}\varphi_{i,3} \varphi_{j,2}+\varphi_{m,2}\varphi_{i,3} \varphi_{j,1} 
      }\nonumber\\
      &\hspace{11mm}-\varphi_{m,2}\varphi_{i,1} \varphi_{j,3}+\varphi_{m,3}\varphi_{i,1} \varphi_{j,2} - \varphi_{m,3}\varphi_{i,2} \varphi_{j,1}
      ) \nonumber\\
  &= \sumlim{i,j=1}{N}{c_{i2}c_{j3} 
      \det \begin{bmatrix}
              \nabla \varphi_{m} \\
              \nabla \varphi_{i} \\
              \nabla \varphi_{j}           
            \end{bmatrix}
     }
  = \nabla_{c_{m1}}\left\{\det \BF(X,t)\right\} \,.
}

