We now collect the $N$ position coefficient vectors $\vc_i \in\R^3$ and pressure coefficients as
\begin{align*}
	\vu(t) &:= (\vc_1^T(t) \ldots \vc_N^T(t))^T \in\R^{3N},\\
	\vw(t) &:= (d_1(t) \ldots d_{N_P}(t))^T \in\R^{N_P}.
\end{align*}
We introduce the triple index
\begin{align}
	[i] &:= 3(i-1)+(1~2~3)^T, \text{ i.e.}\\
	\vu[i] &:= (\vu_{3(i-1)+1}~~\vu_{3(i-1)+2}~~\vu_{3(i-1)+3})^T\in\R^{3\times 1}
\end{align}
for the $x,y,z$ components of the $i$-th coefficient and hence identify
\[
	\vF(X,t) = \sumi \vc_i(t)\otimes \nabla\varphi_i(X) = \sumi \vu[i](t)\otimes \nabla\varphi_i(X) =: \vF(X,\vu(t)).
\]
also carrying the arguments through to $\vP(X,t) = \vP(X,\vu(t),\vw(t))$.
This allows us to define operators $\vK: \R^{3N\times N_P}\to\R^{3N}, \vg:\R^{3N}\to\R^{N_P}$ (by components) as
\begin{align}
	\vK[k](\vu(t),\vw(t)) &:= \intor\vP(X,\vu(t),\vw(t))\dpk dX\\
	&\re{def:discretePgradphidX} \sumvk\sumgp w_p\vP(\pmp,\vu(t),\vw(t))\dNkmp\jmp\in\R^3, && k=1\ldots N,\\
	\vg_k(\vu(t)) &:= \intor (\det\vF(X,\vu(t))-1)\psi_k(X)dX\\
	&\re{eq:weak_incomp_condition}\sumvk\sumgp w_p (\det\vF(\pmp,\vu(t))-1) \Nkmp\jmp, && k=1\ldots N_P.
\end{align}
Furthermore, from \eqref{def:discreteVphidX} we obtain a mass matrix $\vM\in\R^{3N\times 3N}$ via
\begin{align*}
	\vM\bigl[[i],[k]\bigr] &:= \m{1&0&0\\0&1&0\\0&0&1} \sumvk\sumgp w_p \rho_0(\pmp)N_{l(i,m)}(X_p) \Nkmp\jmp, && i,k=1\ldots N.
\end{align*}

Altogether, the system of equations \eqref{def:mainsys1_weak_kparts},\eqref{def:maineq_cond_weak_kparts} yields the constrained second order differential equation
or differential-algebraic equation (DAE)
\begin{align}
	\vM\vu''(t) + \vK(\vu(t),\vw(t)) &= \vnull,\\
		\text{s.t.}\quad \vg(\vu(t)) &= \vnull,
\end{align}
which can be transformed to a first-order system with the substitution $\vv(t) := \vu'(t)$:
\begin{align}
	\m{\vI & \vnull\\ \vnull & \vM}\m{\vu'(t)\\ \vv'(t)} &= \m{\vv(t) \\ -\vK(\vu(t),\vw(t))},\\
	\text{s.t.}\quad \vg(\vu(t))		&= \vnull.
\end{align}

\subsection{Time-discretization}
For the time-discretization we use the notation $\vu_i := \vu(t_i), t_i := i\Delta t, i=0\ldots N_t\in\N, \Delta t > 0$, similarly for $\vv,\vw$.
Using the standard backward-Euler scheme results in the implicit system
\begin{align}
	\frac{1}{\Delta t}\m{\vI & \vnull\\ \vnull & \vM}\m{\vu_{i+1}-\vu_i\\\vv_{i+1}-\vv_i} &= \m{\vv_{i+1}\\-\vK(\vu_{i+1},\vw_{i+1})},\\
	\vg(\vu_{i+1})		&= \vnull.
\end{align}
Writing the overall system as 
\begin{align}
	\vf([\vu; \vv; \vw]) &:= \m{\frac{1}{\Delta t}\m{\vI & \vnull\\ \vnull & \vM}\m{\vu-\vu_i\\\vv-\vv_i} + \m{-\vv\\\vK(\vu,\vw)}\\
		\vg(\vu)},
\end{align}
we apply the standard Newton-Iteration
\begin{align}
	[\vu; \vv; \vw]^1 &:= [\vu_i; \vv_i; \vw_i],\\
	[\vu; \vv; \vw]^{n+1} &:= [\vu; \vv; \vw]^{n} - \nabla \vf([\vu; \vv; \vw]^n)^{-1}\vf([\vu; \vv; \vw]^n), 
\end{align}
to find $\vu_{i+1}$ etc.
Here we have the Jacobian
\begin{align}
	 \nabla \vf([\vu; \vv; \vw]) &:= \m{\frac{1}{\Delta t} \vI & -\vI & \vnull & \Bigl\rbrace3N\\
	 									\nabla_{\vu}\vK(\vu,\vw) & \frac{1}{\Delta t}\vM & \nabla_{\vw}\vK(\vu,\vw) & \Bigl\rbrace3N\\
	 									\underbrace{\nabla_{\vu}\vg(\vu)}_{3N} & \underbrace{\vnull}_{3N} & \underbrace{\vnull}_{N_P} & \Bigl\rbrace N_P}.
\end{align}

\subsection{Derivation of nonlinearity Jacobian}
Here are some important formulas for matrix derivatives. We first define
\begin{align}
    \vU^j_i(X) & := \m{\ve_i\otimes\dpj}, i=1\ldots3, &
	\vU^j_1(X) &= \m{
            ~   & \dpj  & ~ \\
            0   & 0                 & 0 \\
            0   & 0                 & 0
          },\\
  \vU^j_2(X) &= \m{
            0   & 0                 & 0 \\
            ~   & \dpj  & ~ \\            
            0   & 0                 & 0
          },& 
  \vU^j_3(X) & = \m{
            0   & 0                 & 0 \\
            0   & 0                 & 0 \\
            ~   & \dpj  & ~            
          }.
\end{align}
\begin{align}
	\vF(X,\vu + h\ve[j]_i) &= \vF(X,\vu) + \m{\vnull \\ h\dpj^T\\ \vnull}\leftarrow i\nonumber\\
	&= \vF(X,\vu) + h\ve_i\otimes\dpj\\
	&= \vF(X,\vu) + h\vU^j_i(X),\qquad i=1\ldots3,\ve_i\in\R^3 \text{ unit vec}\nonumber\\
	\Rightarrow \d{}{u[j]_i}\vF(X,\vu) &= \vU^j_i(X),\qquad i=1\ldots3\nonumber\\
	(\vS+\Delta\vU)^{-1} &= \vS^{-1} - \vS^{-1}\Delta\vU\vS^{-1} + \O{|\Delta U|^2}\qquad\cite[p.57]{Bonet2008}\label{eq:matrixinversederivative}\\
	\vF(X,\vu + h\ve[j]_i)^{-1} &= \left(\vF(X,\vu) + h\vU^j_i(X)\right)^{-1}\nonumber\\
		&\re{eq:matrixinversederivative}\vF(X,\vu)^{-1} - h\vF(X,\vu)^{-1}\vU^j_i(X)\vF(X,\vu)^{-1} + \O{h^2}\nonumber\\
	\Rightarrow\d{}{u[j]_i}\vF^{-1}(X,\vu) &= -\vF(X,\vu)^{-1}\vU^j_i(X)\vF(X,\vu)^{-1}\nonumber\\
	\Rightarrow\d{}{u[j]_i}\vF^{-T}(X,\vu) &= -\vF(X,\vu)^{-T}(\vU^j_i(X))^{T}\vF(X,\vu)^{-T}\nonumber
\end{align}

In detail, we have
% \begin{align*}
% 	\d{\vF}{\vu[k]}(X,\vu) &= \nabla_{\vu[k]}\vF(X,\vu)\\
% 			&= \nabla_{\vu[k]}\sumi \vu[i] \otimes \dpi = \bullet\otimes\dpk\\
% 	\nabla_{\vu[k]}(\det\vF(X,\vu)-1) &= \det(\vF(X,\vu))\vF(X,\vu)^{-1}:\nabla_{\vu[k]}\vF(X,\vu)\\
% 				&= \det(\vF(X,\vu))\vF(X,\vu)^{-1}:\bullet\otimes\dpk
% \end{align*}
\subsubsection{Derivation of $\nabla_{\vu}\vK(\vu,\vw)$}
\begin{align*}
	\nabla_{\vu}\vK(\vu,\vw) &= \m{\nabla_{\vu}\vK[1](\vu,\vw)\\ \vdots \\ \nabla_{\vu}\vK[N](\vu,\vw)}
	 = \m{\nabla_{\vu[1]}\vK[1](\vu,\vw) & \ldots & \nabla_{\vu[N]}\vK[1](\vu,\vw)\\
	 	\vdots & \ddots & \vdots\\
	   \nabla_{\vu[1]}\vK[N](\vu,\vw) & \ldots & \nabla_{\vu[N]}\vK[N](\vu,\vw)}\\
	\nabla_{\vu[j]}\vK[k](\vu,\vw) &=\m{\d{\vK[k]}{\vu[j]_1}(\vu,\vw) & \ldots & \d{\vK[k]}{\vu[j]_3}(\vu,\vw)}\in\R^{3\times 3},\quad j,k=1\ldots N\\
	\d{\vK[k]}{\vu[j]_i}(\vu,\vw) &= \d{}{\vu[j]_i} \intor\vP(X,\vu,\vw)\dpk dX\\
		&=  \intor\d{\vP}{\vu[j]_i}(X,\vu,\vw) \dpk dX\\
		&= \sumvk\sumgp w_p \d{\vP}{\vu[j]_i}(\pmp,\vu,\vw) \dNkmp\jmp\in\R^3
\end{align*}
Recall from \eqref{def:completeP} that
\begin{align*}
\vP(X,\vu,\vw) &= p(X,\vw)\vF^{-T}(X,\vu) + 2(c_{10} + I_1(\vC(X,\vu))c_{01})\vF(X,\vu) - 2c_{01}\vF(X,\vu)\vC(X,\vu)\\
	     &\quad+g(\lambda_f(X,\vu))\vF(X,\vu)\va_0(X)\otimes\va_0(X)
\end{align*}
we consider the single summands of $\vP$ to derive $\d{\vP}{\vu[j]_i}(X,\vu,\vw)$:
\begin{align*}
	 \d{}{\vu[j]_i}p(X,\vw)\vF^{-T}(X,\vu) &= -p(X,\vw)\vF(X,\vu)^{-T}(\dpj\otimes\ve_i)\vF(X,\vu)^{-T}\in\R^{3\times 3}
\end{align*}
\begin{align*}
	\nabla_{\vu[j]}I_1(\vC(X,\vu)) &\re{eq:I1_basis} \nabla_{\vu[j]}\suml{i,l}{N} (\vu[i] \cdot \vu[l])(\dpi \cdot \divergence\varphi_l(X))\\
	&= 2\suml{i}{N} \vu[i](\dpi \cdot \dpj) \in\R^3
\end{align*}
\begin{align*}	 
	 &\d{}{\vu[j]_i}2(c_{10} + I_1(\vC(X,\vu))c_{01})\vF(X,\vu)\\
	 =& 2\d{}{\vu[j]_i}I_1(\vC(X,\vu))c_{01}\vF(X,\vu) + 2(c_{10} + I_1(\vC(X,\vu))c_{01})\d{}{\vu[j]_i}\vF(X,\vu)\\
	 =& 2c_{01}\suml{l}{N} \vu[l]_i(\divergence\varphi_l(X) \cdot \dpj)\vF(X,\vu)\\
	 &+ 2(c_{10} + I_1(\vC(X,\vu))c_{01})\vU^j_i(X)\in\R^{3\times 3}
\end{align*}
\begin{align*}
	\d{}{\vu[j]_i}\vC(X,\vu) &= \d{}{\vu[j]_i}\suml{m,l}{N} (\vu[m] \cdot \vu[l])(\divergence\varphi_m(X) \otimes \divergence\varphi_l(X))\\
	&= 2\suml{l}{N} \vu[l]_i(\dpj \otimes \divergence\varphi_l(X))\in\R^{3\times 3}
\end{align*}
\begin{align*}
	&\d{}{\vu[j]_i}2c_{01}\vF(X,\vu)\vC(X,\vu)\\
	=& 2c_{01}\left(\left(\d{}{\vu[j]_i}\vF(X,\vu)\right)\vC(X,\vu) + \vF(X,\vu)\d{}{\vu[j]_i}\vC(X,\vu)\right)\\
	=& 2c_{01}\left(\left(\vU^j_i(X)\right)\vC(X,\vu)
	+ 2\vF(X,\vu)\suml{l}{N} \vu[l]_i(\dpj \otimes \divergence\varphi_l(X))\right)\in\R^{3\times 3}
\end{align*}
\begin{align*}
	\nabla_{\vu[j]}\lambda_f(X,\vu) &= \nabla_{\vu[j]}\sqrt{\suml{m,l}{N} (\vu[m] \cdot \vu[l])\left(\divergence\varphi_m(X)\cdot a_0(X)\right)(\divergence\varphi_l(X)\cdot a_0(X))}\\
	&= \frac{1}{2\lambda_f(X,\vu)} \nabla_{\vu[j]}\suml{m,l}{N} (\vu[m] \cdot \vu[l])\left(\divergence\varphi_m(X)\cdot a_0(X)\right)(\divergence\varphi_l(X)\cdot a_0(X))\\
	&= \frac{1}{2\lambda_f(X,\vu)} 2\suml{l}{N} \vu[l]\left(\dpj\cdot a_0(X)\right)(\divergence\varphi_l(X)\cdot a_0(X))\\
	&= \frac{1}{\lambda_f(X,\vu)} \suml{l}{N} \vu[l]\left(\dpj\cdot a_0(X)\right)(\divergence\varphi_l(X)\cdot a_0(X))
\end{align*}
\begin{align*}
	  & \d{}{\vu[j]_i} g(\lambda_f(X,\vu))\vF(X,\vu)\va_0(X)\otimes\va_0(X)\\
	 =& \left( \d{g}{\lambda_f}(\lambda_f(X,\vu))\d{}{\vu[j]_i}\lambda_f(X,\vu)\vF(X,\vu) + g(\lambda_f(X,\vu))\ve_i\otimes\dpj\right)\va_0(X)\otimes\va_0(X) 
\end{align*}
\begin{align*}
	  f_l'(\lambda) &\re{def:fl} \begin{cases}
		\frac{12.5}{\lfo}\left(1-\frac{\lambda_f}{\lfo}\right) & 0.6 \leq \frac{\lambda_f}{\lfo} \leq 1.4\\ 
		0 & \text{else}
	\end{cases}\\	
	   \d{g}{\lambda_f} &\re{def:g} \d{}{\lambda_f}\left(\frac{b_1}{\lambda_f^2}\left(\lambda_f^{d_1} - 1\right)
		+\frac{p^{max}}{\lambda_f}f_l(\lambda_f)\gamma\left(\alpha,\d{\lambda_f}{t}\right)\right)\\
		&= -\frac{b_1}{\lambda_f^3}\left(\lambda_f^{d_1} - 1\right) + \frac{b_1}{\lambda_f^2}(d_1-1)\lambda_f^{d_1-1}
		+p^{max}\gamma\left(\alpha,\d{\lambda_f}{t}\right) \left(-\frac{1}{\lambda_f^2}f_l(\lambda_f) + \frac{1}{\lambda_f}f_l'(\lambda_f)\right)\\
		&= \frac{b_1}{\lambda_f^3}\left((d_1-1)\lambda_f^{d_1} - (\lambda_f^{d_1} - 1)\right)
		+p^{max}\gamma\left(\alpha,\d{\lambda_f}{t}\right) \left(-\frac{1}{\lambda_f^2}f_l(\lambda_f) + \frac{1}{\lambda_f}f_l'(\lambda_f)\right)\\
		&= \frac{b_1}{\lambda_f^3}\left((d_1-2)\lambda_f^{d_1} + 2\right)
		+p^{max}\gamma\left(\alpha,\d{\lambda_f}{t}\right) \left(-\frac{1}{\lambda_f^2}f_l(\lambda_f) 
		+ \underbrace{\frac{12.5}{\lambda_f\lfo}\left(1-\frac{\lambda_f}{\lfo}\right)}_{\neq 0\text{ if }0.6 \leq \frac{\lambda_f}{\lfo} \leq 1.4}\right)\\
		&= \frac{b_1}{\lambda_f^3}\left((d_1-2)\lambda_f^{d_1} + 2\right)
		+ \frac{p^{max}}{\lambda_f^2}\gamma\left(\alpha,\d{\lambda_f}{t}\right) \left( 
		\underbrace{12.5\frac{\lambda_f}{\lfo}\left(1-\frac{\lambda_f}{\lfo}\right)}_{\neq 0\text{ if }0.6 \leq \frac{\lambda_f}{\lfo} \leq 1.4}-f_l(\lambda_f)\right)
\end{align*}

\subsubsection{Derivation of $\nabla_{\vw}\vK(\vu,\vw)$}
\begin{align*}
	\nabla_{\vw}\vK(\vu,\vw) &= \m{\nabla_{\vw}\vK[1](\vu,\vw)\\ \vdots \\ \nabla_{\vw}\vK[N](\vu,\vw)}
	 = \m{\d{\vK[1]}{\vw_1}(\vu,\vw) & \ldots & \d{\vK[1]}{\vw_N}(\vu,\vw)\\
	 	\vdots & \ddots & \vdots\\
	   \d{\vK[N]}{\vw_1}(\vu,\vw) & \ldots & \d{\vK[N]}{\vw_N}(\vu,\vw)}\\
	\d{\vK[k]}{\vw_i}(\vu,\vw) &= \d{}{\vw_i} \intor\vP(X,\vu,\vw)\dpk dX\\
		&=  \intor\d{}{\vw_i} \left[p\vF^{-T}(X,\vu) +[\ldots] \right] \dpk dX\\
		&=  \intor\d{}{d_i} \left[\sumi d_j\psi_j(X)\vF^{-T}(X,\vu) +[\ldots] \right] \dpk dX\\
		&=  \intor \psi_i(X)\vF^{-T}(X,\vu)\dpk dX\\
		&= \sumvk\sumgp w_p \psi_i(\pmp)\vF^{-T}(\pmp,\vu) \dNkmp\jmp\in\R^3
\end{align*}

\subsubsection{Derivation of $\nabla_{\vu}\vg(\vu)$}
\begin{align*}
	\nabla_{\vu}\vg(\vu) &= \m{\nabla_{\vu}\vg_1(\vu)\\ \vdots \\ \nabla_{\vu}\vg_M(\vu)}
	 = \m{\d{\vg_1}{\vu[1]}(\vu) & \ldots & \d{\vg_1}{\vu[N]}(\vu)\\
	 	\vdots & \ddots & \vdots\\
	   \d{\vg_M}{\vu[1]}(\vu) & \ldots & \d{\vg_M}{\vu[N]}(\vu)} \in\R^{M \times 3N}\\
	\nabla_{\vu[j]}\vg_k(\vu) &= \nabla_{\vu[j]}\intor (\det\vF(X,\vu)-1)\psi_k(X)dX\qquad\in\R^{1\times 3}\\
		&\re{eq:weak_incomp_condition}  \sumvk\sumgp w_p \nabla_{\vu[j]}\det\vF(\pmp,\vu)\Nkmp\jmp\\
		&= \sumvk\sumgp w_p \det\vF(\pmp,\vu)\m{\vF(\pmp,\vu)^{-T}:\vU(\pmp)^j_1\\\vF(\pmp,\vu)^{-T}:\vU(\pmp)^j_2\\\vF(\pmp,\vu)^{-T}:\vU(\pmp)^j_3}^TN_{l(k,m)}(X_p)\jmp\\
		&= \sumvk\sumgp w_p \det\vF(\pmp,\vu)\m{\tr(\vF(\pmp,\vu)^{-1}\vU(\pmp)^j_1)\\\tr(\vF(\pmp,\vu)^{-1}\vU(\pmp)^j_2)\\\tr(\vF(\pmp,\vu)^{-1}\vU(\pmp)^j_3)}^TN_{l(k,m)}(X_p)\jmp\in\R^{1\times 3}
\end{align*}



